theories/Term.v
@@ -1,6 +1,5 @@
 From LinearCore Require
   Constructor
-  Name
   Pattern
   .
 From LinearCore Require Import
@@ -12,10 +11,10 @@ From LinearCore Require Import
 (* TODO: make `Err`, `Typ`, & `Prp` constructors? *)
 Inductive term : Set :=
   | Ctr (constructor : Constructor.constructor)
-  | Mov (name : Name.name)
-  | Ref (name : Name.name)
+  | Mov (name : String.string)
+  | Ref (name : String.string)
   | App (function : term) (argument : term)
-  | For (variable : Name.name) (type : term) (body : term)
+  | For (variable : String.string) (type : term) (body : term)
   | Cas (pattern : Pattern.pattern) (body_if_match : term) (other_cases : term)
   .
 
@@ -23,9 +22,9 @@ Fixpoint eq a b :=
   match a, b with
   | Ctr a, Ctr b => Constructor.eq a b
   | Mov a, Mov b
-  | Ref a, Ref b => Name.eqb a b
+  | Ref a, Ref b => String.eqb a b
   | App fa aa, App fb ab => andb (eq fa fb) (eq aa ab)
-  | For va ta ba, For vb tb bb => andb (Name.eqb va vb) (andb (eq ta tb) (eq ba bb))
+  | For va ta ba, For vb tb bb => andb (String.eqb va vb) (andb (eq ta tb) (eq ba bb))
   | Cas pa ba oa, Cas pb bb ob => andb (Pattern.eq pa pb) (andb (eq ba bb) (eq oa ob))
   | _, _ => false
   end.
@@ -37,13 +36,13 @@ Proof.
   try (constructor; intro D; discriminate D); try (constructor; reflexivity).
   - unfold eq. destruct (Constructor.eq_spec constructor constructor0); constructor. { f_equal. assumption. }
     intro E. apply N. invert E. reflexivity.
-  - simpl eq. destruct (Name.spec name name0); constructor. { f_equal. assumption. }
-    intro E. apply N. invert E. reflexivity.
-  - simpl eq. destruct (Name.spec name name0); constructor. { f_equal. assumption. }
-    intro E. apply N. invert E. reflexivity.
+  - simpl eq. destruct (String.eqb_spec name name0); constructor. { f_equal. assumption. }
+    intro E. apply n. invert E. reflexivity.
+  - simpl eq. destruct (String.eqb_spec name name0); constructor. { f_equal. assumption. }
+    intro E. apply n. invert E. reflexivity.
   - simpl eq. destruct (IHa1 b1); cbn. 2: { constructor. intro E. apply N. invert E. reflexivity. }
     subst. destruct (IHa2 b2); constructor. { f_equal. assumption. } intro E. apply N. invert E. reflexivity.
-  - simpl eq. destruct (Name.spec variable variable0); cbn in *. 2: { constructor. intro E. apply N. invert E. reflexivity. }
+  - simpl eq. destruct (String.eqb_spec variable variable0); cbn in *. 2: { constructor. intro E. apply n. invert E. reflexivity. }
     destruct (IHa1 b1); cbn. 2: { constructor. intro E. apply N. invert E. reflexivity. }
     subst. destruct (IHa2 b2); constructor. { f_equal. assumption. } intro E. apply N. invert E. reflexivity.
   - simpl eq. destruct (Pattern.eq_spec pattern pattern0); cbn in *. 2: { constructor. intro E. apply N. invert E. reflexivity. }
@@ -58,9 +57,9 @@ From Coq Require Import String.
 Fixpoint to_string t : string :=
   match t with
   | Ctr ctor => Constructor.to_string ctor
-  | Mov name => Name.to_string name
-  | Ref name => "&" ++ Name.to_string name
+  | Mov name => name
+  | Ref name => "&" ++ name
   | App function argument => "(" ++ to_string function ++ ") (" ++ to_string argument ++ ")"
-  | For variable type body => "forall (" ++ Name.to_string variable ++ ": " ++ to_string type ++ "), " ++ to_string body
+  | For variable type body => "forall " ++ variable ++ ": " ++ to_string type ++ ", " ++ to_string body
   | Cas pattern body_if_match other_cases => "if match " ++ Pattern.to_string pattern ++ " then { " ++ to_string body_if_match ++ " } else " ++ to_string other_cases
   end.
