theories/Context.v
@@ -2,6 +2,9 @@ From LinearCore Require
   Map
   Term
   .
+From LinearCore Require Import
+  DollarSign
+  .
 
 
 
@@ -12,7 +15,7 @@ Arguments context/.
 
 From Coq Require Import String.
 
-Definition format_pair kv : string := Name.to_string (fst kv) ++ " -> " ++ Term.to_string (snd kv).
+Definition format_pair kv : string := fst kv ++ " -> " ++ Term.to_string $ snd kv.
 
 Definition to_string ctx : string :=
-  "{ " ++ String.concat "; " (List.map format_pair (MapCore.bindings ctx)) ++ "}".
+  "{ " ++ String.concat "; " (List.map format_pair $ MapCore.bindings ctx) ++ "}".
